state/README.md
@@ -1,0 +1,4 @@
+# TODO: prove assumptions
+* `lemma_modifies_only_label_trans` in `IFC.Heap.ST`
+* `write'`, `_alloc`, `declassify_low'`, `alloc'` in `TargetLangIFC` --- one could use the same strategy to prove all of them
+* `inversion` in `TargetLangIFC` --- we cannot prove this without some workarounds
